make specialized boardrm for extraction, fix in liq extraction

extraction/examples/BoardroomVotingExtraction.v
@@ -5,7 +5,7 @@
 From Coq Require Import PeanoNat ZArith.
 
 From ConCert.Extraction Require Import LPretty LiquidityExtract Common.
-From ConCert.Execution Require Import Blockchain Common.
+From ConCert.Execution Require Import Blockchain Common LocalBlockchain.
 
 From Coq Require Import List String.
 Local Open Scope string_scope.
@@ -20,143 +20,109 @@ Open Scope Z.
 
 Definition PREFIX := "".
 
-From ConCert.Execution.Examples Require Import BoardroomVotingTest.
-Import Params.
+From ConCert.Execution.Examples Require Import BoardroomVotingZ.
+
+(* In this example we just use xor for the hash function, which is
+   obviously not cryptographically secure. *)
+Definition modulus : Z := 201697267445741585806196628073.
+Definition four := 4%nat.
+Definition seven := 7%nat.
+Definition _1234583932 := 1234583932.
+Definition _23241 := 23241.
+Definition _159338231 := 159338231.
+Definition oneN : N := 1%N.
+Definition Z3 : Z := 3.
+Definition generator : Z := Z3.
+
+Definition hash_func (l : list positive) : positive :=
+  N.succ_pos (fold_left (fun a p => N.lxor (Npos p) a) l oneN).
+
+  (* Instance Base : ChainBase := LocalChainBase AddrSize. *)
+Definition AddrSize := (2^128)%N.
+Instance Base : ChainBase := LocalBlockchain.LocalChainBase AddrSize.
+
+Module Params <: BoardroomParams.
+  Definition H : list positive -> positive := hash_func.
+  Definition Base := Base .
+  Definition prime := modulus.
+  Definition generator := generator.
+End Params.  
+Module BV := BoardroomVoting Params. Import BV.
+
+(* Compute the signup messages that would be sent by each party.
+   We just use the public key as the chosen randomness here. *)
+Definition _3 := 3%nat.
+Definition _5 := 5.
+Definition _11 := 11.
+
+Definition num_parties : nat := seven.
+Definition votes_for : nat := four.
+
+(* a pseudo-random generator for secret keys *)
+Definition sk n := (Z.of_nat n + _1234583932) * (modulus - _23241)^_159338231.
+
+(* Make a list of secret keys, here starting at i=7 *)
+Definition sks : list Z := map sk (seq seven num_parties).
+
+(* Make a list of votes for each party *)
+Definition svs : list bool :=
+  Eval compute in map (fun _ => true)
+                      (seq 0 votes_for)
+                  ++ map (fun _ => false)
+                         (seq 0 (num_parties - votes_for)).
+
+(* Compute the public keys for each party *)
+(* 
+Time Definition pks : list Z :=
+  Eval vm_compute in map compute_public_key sks.
+
+Definition rks : list Z :=
+  Eval vm_compute in map (reconstructed_key pks) (seq 0 (length pks)).
+
+Time Definition signups : list Msg :=
+  Eval vm_compute in map (fun '(sk, pk, i) => make_signup_msg sk _5 i)
+                             (Extras.zip (zip sks pks) (seq 0 (length sks))).
+
+(* Compute the submit_vote messages that would be sent by each party *)
+(* Our functional correctness proof assumes that the votes were computed
+   using the make_vote_msg function provided by the contract.
+   In this example we just use the secret key as the random parameters. *)
+Definition votes : list Msg :=
+  Eval vm_compute in map (fun '(i, sk, sv, rk) => make_vote_msg pks i sk sv sk sk sk)
+                             (zip (zip (zip (seq 0 (length pks)) sks) svs) rks).
+
+Definition A a :=
+  BoundedN.of_Z_const AddrSize a.
+
+Local Open Scope nat.
+Definition addrs : list Address.
+Proof.
+  let rec add_addr z n :=
+    match n with
+    | O => constr:(@nil Address)
+    | S ?n => let tail := add_addr (z + 1)%Z n in
+              constr:(cons (A z) tail)
+    end in
+  let num := eval compute in num_parties in
+  let tm := add_addr _11%Z num in
+  let tm := eval vm_compute in tm in
+  exact tm.
+Defined.
+
+Definition voters_map : AddrMap unit := AddressMap.of_list (map (fun a => (a, tt)) addrs).
+
+Definition five := 5%nat.
+
+Definition deploy_setup :=
+  {| eligible_voters := voters_map;
+     finish_registration_by := _3;
+     finish_commit_by := None;
+     finish_vote_by := five;
+     registration_deposit := 0; |}. *)
+
 (* Get string representation of modulus, and remap it. This way we avoid having the extraction compute the number. *)
-Definition modulus_ := StringExtra.string_of_Z BoardroomVotingTest.modulus.
+Definition modulus_ := StringExtra.string_of_Z modulus.
 
-Print BoardroomMath.BoardroomAxioms.
-(* TODO: remap all definition in boardroomaxioms *)
-(* Definition TT_boardroomaxioms : list (kername * string) :=
-  [
-    elmeqb_spec : 
-    zero 
-    one 
-    add : A -> A -
-    mul : A -> A -
-    opp : A -
-    inv : A -
-    pow : A -> Z -
-    order 
-    expeq := fun e e' : Z => e mod (order - 1) = e' mod (order - 
-    order_ge_2 : order >
-  ] *)
-Print Params.
-  Definition eqlemeqb_Z := @BoardroomMath.elmeqb _ Params.axioms.
-  
-  (* elmeq a b := a mod p = b mod p;
-     elmeqb a b := a mod p =? b mod p;
-     zero := 0;
-     one := 1;
-     add a a' := (a + a') mod p;
-     mul a a' := (a * a') mod p;
-     opp a := p - a;
-     inv a := Zp.mod_inv a p;
-     pow a e := Zp.mod_pow a e p;
-     order := p; *)
-
-(** A translation table for definitions we want to remap. The corresponding top-level definitions will be *ignored* *)
-Definition TT_remap : list (kername * string) :=
-  TT_remap_default ++ [
-    remap <%% Amount %%> "tez"
-  ;  remap <%% positive %%> "nat"
-  ; remap <%% Z %%> "int"
-  ; remap <%% Z.of_nat %%> "%int"
-  ; remap <%% Z.add %%> "addInt"
-  ; remap <%% Z.sub %%> "subInt"
-  ; remap <%% Z.leb %%> "leInt"
-  ; remap <%% Z.ltb %%> "ltInt"
-  ; remap <%% Z.add %%> "addInt"
-  ; remap <%% Z.eqb %%> "eqInt"
-  ; remap <%% Z.gtb %%> "gtbInt"
-  ; remap <%% Nat.ltb %%> "ltbNat"
-  ; remap <%% Z.modulo %%> "modInt"
-  ; remap <%% Z.mul %%> "mulInt"
-  ; remap <%% N.lxor %%> "xor"
-  ; remap <%% N.succ_pos %%> "(addNat 1)"
-
-  ; remap <%% BoardroomVotingTest.oneN %%> "1"
-  ; remap <%% BoardroomVotingTest.four %%> "4"
-  ; remap <%% BoardroomVotingTest.seven %%> "7"
-  ; remap <%% BoardroomVotingTest._1234583932 %%> "1234583932"
-  ; remap <%% BoardroomVotingTest._23241 %%> "23241"
-  ; remap <%% BoardroomVotingTest._159338231 %%> "159338231"
-  ; remap <%% BoardroomVotingTest._5 %%> "5"
-  ; remap <%% BoardroomVotingTest._3 %%> "3"
-  ; remap <%% BoardroomVotingTest._11 %%> "11"
-  ; remap <%% BoardroomVotingTest.five %%> "5"
-  ; remap <%% @ContractCallContext %%> "(address * (address * int))"
-  ; remap <%% @Chain %%> "(address * (address * address))" (* chain_height, current_slot, finalized_height *)
-  ; remap <%% @chain_height %%> "fst" (* small hack, but valid since ContractCallContext is mapped to a tuple *)
-  ; remap <%% @current_slot %%> "(fun c -> fst (snd c)" (* small hack, but valid since Chain is mapped to a tuple *)
-  ; remap <%% @finalized_height %%> "(fun c -> snd (snd c)" (* small hack, but valid since Chain is mapped to a tuple *)
-  ; remap <%% @ctx_from %%> "fst" (* small hack, but valid since ContractCallContext is mapped to a tuple *)
-  ; remap <%% @AddressMap.AddrMap %%> "addrMap"
-  ; remap <%% @AddressMap.add %%> "Map.add"
-  ; remap <%% @AddressMap.find %%> "Map.find"
-  ; remap <%% @AddressMap.values %%> "Map.to_list"
-  ; remap <%% @AddressMap.empty %%> "(Map [])"
-
-  ; remap <%% BoardroomMath.Zp.mod_pow %%> "mod_powInt"
-  ; remap <%% BoardroomMath.Zp.mod_inv %%> "mod_invInt"
-  (*; remap <%% @BoardroomMath.add%%> "addInt"
-  ; remap <%% @BoardroomMath.elmeq%%> "eqInt"
-  ; remap <%% @BoardroomMath.expeq%%> "expeq"
-  ; remap <%% @BoardroomMath.elmeqb%%> "eqInt"
-  ; remap <%% @BoardroomMath.zero%%> "0"
-  ; remap <%% @BoardroomMath.one%%> "1"
-  ; remap <%% @BoardroomMath.mul%%> "mulInt"
-  ; remap <%% @BoardroomMath.opp%%> "-"
-  ; remap <%% @BoardroomMath.inv%%> "inv"
-  ; remap <%% @BoardroomMath.pow%%> "pow"
-  ; remap <%% @BoardroomMath.order%%> "order"
-  ; remap <%% @BoardroomVotingTest.axioms%%> "" *)
-
-  (* ; remap <%% BV.verify_secret_vote_proof %%> "verify_secret_vote_proof" *)
-  (* ; remap <%% @BV.make_signup_msg %%> "make_signup_msg" *)
-  (* ; remap <%% @BV.make_commit_msg %%> "make_commit_msg" *)
-  (* ; remap <%% @BV.make_vote_msg %%> "make_vote_msg" *)
-  (* ; remap <%% @BV.secret_vote_proof %%> "secret_vote_proof" *)
-  (* ; remap <%% @BV.secret_key_proof %%> "secret_key_proof" *)
-  (* ; remap <%% @BV.hash_sk_data %%> "hash_sk_data" *)
-  (* ; remap <%% @BV.hash_sv_data %%> "hash_sv_data" *)
-
-  (* ; remap <%% @BV.handle_signup %%> "handle_signup" *)
-  ; remap <%% @BV.handle_commit_to_vote %%> "handle_commit_to_vote"
-  ; remap <%% @BV.handle_submit_vote %%> "handle_submit_vote"
-  ; remap <%% @BV.handle_tally_votes %%> "handle_tally_votes"
-
-
-  ; remap <%% BoardroomVotingTest.modulus %%> modulus_
-  ; remap <%% @modulus_prime %%> "modulus_prime"
-  ; remap <%% BV.encodeA %%> "%nat"
-  ; remap <%% BV.encodeNat %%> "%nat"
-  
-
-  ; remap <%% @List.fold_left %%> "List.fold"
-  ; remap <%% @List.map %%> "List.map"
-  ; remap <%% @List.find %%> "List.find"
-  ; remap <%% @List.length %%> "List.length"
-  ; remap <%% @List.app %%> "List.append"
-  ; remap <%% @Serializable.serialize %%> "TODO_serialize"
-  ; remap <%% @Serializable.deserialize %%> "TODO_deserialize"
-  ].
-(** A translation table of constructors and some constants. The corresponding definitions will be extracted and renamed. *)
-Definition TT_rename : list (string * string):=
-  [ ("Some", "Some")
-  ; ("None", "None")
-  ; ("Zpos" ,"%int")
-  ; ("Npos" ,"(fun (n:nat) -> n)")
-  ; ("Zneg" ,"-")
-  ; ("Z0" ,"0")
-  ; ("N0" ,"0")
-  ; ("xH" ,"0")
-  ; ("1" ,"1")
-  ; ("nil", "[]")
-  ; ("true", "true")
-  ; (string_of_kername <%% BV.State %%>, "State")  (* we add [storage] so it is printed without the prefix *) 
-  ; ("tt", "()")
-  ].
 Require Import ContractMonads.
 
 Definition init_ctx := (Chain × ContractCallContext).
@@ -174,9 +140,10 @@ Definition receive_wrapper (msg : msg)
   end.
 
 Definition dummy_init : init_ctx -> BV.Setup -> option BV.State := fun _ _ => None .
+
 Definition dummy_receive : msg -> BV.State -> option (list ActionBody × BV.State) := 
   fun _ _  => 
-    let x := BV.secret_key_proof 0 _5 five in
+    let x := add_p 0 _5 in
     None.
 
 Definition BV_MODULE : LiquidityMod msg init_ctx BV.Setup BV.State ActionBody :=
@@ -184,16 +151,16 @@ Definition BV_MODULE : LiquidityMod msg init_ctx BV.Setup BV.State ActionBody :=
     lmd_module_name := "liquidity_boardroomvoting" ;
 
     (* definitions of operations on pairs and ints *)
-    lmd_prelude := concat nl [prod_ops;int_ops];
+    lmd_prelude := LiquidityPrelude;
 
     (* initial storage *)
-    lmd_init := dummy_init ;
+    lmd_init := init_wrapper;
 
     (* no extra operations in [init] are required *)
     lmd_init_prelude := "" ;
 
     (* the main functionality *)
-    lmd_receive := dummy_receive;
+    lmd_receive := receive_wrapper;
 
     (* code for the entry point *)
     lmd_entry_point := printWrapper (PREFIX ++ "receive_wrapper") ++ nl
@@ -203,79 +170,11 @@ Definition BV_MODULE : LiquidityMod msg init_ctx BV.Setup BV.State ActionBody :=
     It uses the certified erasure from [MetaCoq] and the certified deboxing procedure
     that removes application of boxes to constants and constructors. *)
 (* Require Import RecordSet. *)
-Print Params.
+
 Definition inline_boardroom_params : list kername :=
   [
-      <%% Params.A %%>
-    ; <%% Params.H %%>
-    ; <%% Params.ser %%>
-    (* ; <%% Params.axioms %%> *)
-    ; <%% Params.gen %%>
-    ; <%% Params.discr_log %%>
-    (* ; <%% BoardroomVotingTest.axioms_instance %%> *)
-    (* ; <%% BVZAxioms.boardroom_axioms_Z %%> *)
-
-    (* ; <%% @BoardroomMath.oeq_equivalence %%> *)
-    (* ; <%% @BoardroomMath.generator_instance %%> *)
-    (* ; <%% @BoardroomMath.generator %%> *)
-    (* ; <%% @BoardroomMath.generator_nonzero %%> *)
-    (* ; <%% @BoardroomMath.generator_generates %%> *)
-    (* ; <%% @BoardroomMath.log %%>
-    ; <%% @BoardroomMath.log_proper %%>
-    ; <%% @BoardroomMath.log_1_l %%>
-    ; <%% @BoardroomMath.log_generator %%> *)
-
-    (* BoardroomAxioms *)
-    (* ; <%% @BoardroomMath.BoardroomAxioms%%>
-    ; <%% @BoardroomMath.add%%>
-    ; <%% @BoardroomMath.elmeq%%>
-    ; <%% @BoardroomMath.expeq%%>
-    ; <%% @BoardroomMath.elmeqb%%>
-    ; <%% @BoardroomMath.zero%%>
-    ; <%% @BoardroomMath.one%%>
-    ; <%% @BoardroomMath.mul%%>
-    ; <%% @BoardroomMath.opp%%>
-    ; <%% @BoardroomMath.inv%%>
-    ; <%% @BoardroomMath.pow%%>
-    ; <%% @BoardroomMath.order%%> *)
-
-    (* ; <%% @BoardroomMath.plus_expeq_proper%%>
-    ; <%% @BoardroomMath.mul_expeq_proper%%>
-    ; <%% @BoardroomMath.sub_expeq_proper%%>
-    ; <%% @BoardroomMath.opp_expeq_proper%%>
-    ; <%% @BoardroomMath.pow_generator_proper%%>
-    ; <%% @BoardroomMath.prod_perm_proper%%>
-    ; <%% @BoardroomMath.bruteforce_tally_aux_proper%%>
-    ; <%% @BoardroomMath.bruteforce_tally_proper%%>
-    ; <%% @BoardroomMath.elmeqb_elmeq_proper%%>
-
-    ; <%% @BoardroomMath.elmeqb_spec%%>
-    ; <%% @BoardroomMath.order_ge_2%%>
-    ; <%% @BoardroomMath.elmeq_equiv%%>
-    ; <%% @BoardroomMath.add_proper%%>
-    ; <%% @BoardroomMath.mul_proper%%>
-    ; <%% @BoardroomMath.opp_proper%%>
-    ; <%% @BoardroomMath.inv_proper%%>
-    ; <%% @BoardroomMath.pow_base_proper%%>
-    ; <%% @BoardroomMath.pow_exp_proper%%>
-    ; <%% @BoardroomMath.one_neq_zero%%>
-    ; <%% @BoardroomMath.add_comm %%>
-    ; <%% @BoardroomMath.add_assoc %%>
-    ; <%% @BoardroomMath.mul_comm %%>
-    ; <%% @BoardroomMath.mul_assoc %%>
-    ; <%% @BoardroomMath.add_0_l %%>
-    ; <%% @BoardroomMath.mul_0_l %%>
-    ; <%% @BoardroomMath.mul_1_l %%>
-    ; <%% @BoardroomMath.opp_inv_l %%>
-    ; <%% @BoardroomMath.inv_inv_l %%>
-    ; <%% @BoardroomMath.mul_add %%>
-    ; <%% @BoardroomMath.pow_0_r %%>
-    ; <%% @BoardroomMath.pow_1_r %%>
-    ; <%% @BoardroomMath.pow_opp_1 %%>
-    ; <%% @BoardroomMath.pow_plus %%>
-    ; <%% @BoardroomMath.pow_pow %%>
-    ; <%% @BoardroomMath.pow_nonzero %%>
-    ; <%% @BoardroomMath.inv_nonzero %%> *)
+      <%% Params.H %%>
+    ; <%% Params.generator %%>
   ].
 
 
@@ -306,6 +205,9 @@ Definition to_inline : list kername :=
   ++ [
     <%% Monads.Monad_option %%>
   (* ; <%% @Monads.MonadTrans %%> *)
+  
+  ; <%% ContractIniterSetupState %%>
+  ; <%% ContractReceiverStateMsgState %%>
   ; <%% @contract_initer_monad %%>
   ; <%% @run_contract_initer %%>
   ; <%% @contract_receiver_monad %%>
@@ -361,6 +263,115 @@ inr
   "Erased environment is not expanded enough for dearging to be provably correct"
   : string + string
 *)
+
+(* Time MetaCoq Run ('(env, init_nm, receive_nm) <- quote_and_preprocess to_inline BV_MODULE ;;
+                  tmDefinition "bv_env" env ;;
+                  tmDefinition "bv_init_nm" init_nm ;;
+                  tmDefinition "bv_receive_nm" receive_nm). *)
+
+
+(** A translation table for definitions we want to remap. The corresponding top-level definitions will be *ignored* *)
+Definition TT_remap : list (kername * string) :=
+  (* TT_remap_default ++  *)
+  [
+    remap <%% Amount %%> "tez"
+  ; remap <%% positive %%> "nat"
+  ; remap <%% Z %%> "int"
+  ; remap <%% Z.of_nat %%> "int"
+  ; remap <%% Z.add %%> "addInt"
+  ; remap <%% Z.sub %%> "subInt"
+  ; remap <%% Z.leb %%> "leInt"
+  ; remap <%% Z.ltb %%> "ltInt"
+  ; remap <%% Z.add %%> "addInt"
+  ; remap <%% Z.eqb %%> "eqInt"
+  ; remap <%% Z.gtb %%> "gtbInt"
+  ; remap <%% Nat.ltb %%> "ltbNat"
+  ; remap <%% Z.modulo %%> "modInt"
+  ; remap <%% Z.mul %%> "mulInt"
+  (* ; remap <%% Z.pow %%> "powInt" *)
+  ; remap <%% N.lxor %%> "lxorNat"
+  ; remap <%% N.succ_pos %%> "(addNat 1)"
+  ; remap <%% mod_pow %%> "mod_pow"
+  ; remap <%% Egcd.egcd %%> "egcd"
+  (* ; remap <%% List.nth %%> "List.nth" *)
+  (* ; remap <%% List.firstn %%> "List.firstn" *)
+  (* ; remap <%% List.skipn %%> "List.skipn" *)
+
+  ; remap <%% oneN %%> "1"
+  ; remap <%% four %%> "4"
+  ; remap <%% seven %%> "7"
+  ; remap <%% _1234583932 %%> "1234583932"
+  ; remap <%% _23241 %%> "23241"
+  ; remap <%% _159338231 %%> "159338231"
+  ; remap <%% _5 %%> "5"
+  ; remap <%% _3 %%> "3"
+  ; remap <%% Z3 %%> "3"
+  ; remap <%% _11 %%> "11"
+  (* ; remap <%% five %%> "5" *)
+  ; remap <%% @ContractCallContext %%> "(address * (address * int))"
+  ; remap <%% @Chain %%> "(address * (address * address))" (* chain_height, current_slot, finalized_height *)
+  ; remap <%% @chain_height %%> "fst" (* small hack, but valid since ContractCallContext is mapped to a tuple *)
+  ; remap <%% @current_slot %%> "(fun c -> fst (snd c)" (* small hack, but valid since Chain is mapped to a tuple *)
+  ; remap <%% @finalized_height %%> "(fun c -> snd (snd c)" (* small hack, but valid since Chain is mapped to a tuple *)
+  ; remap <%% @ctx_from %%> "fst" (* small hack, but valid since ContractCallContext is mapped to a tuple *)
+  ; remap <%% @AddressMap.AddrMap %%> "addrMap"
+  ; remap <%% @AddressMap.add %%> "Map.add"
+  ; remap <%% @AddressMap.find %%> "Map.find"
+  ; remap <%% @AddressMap.values %%> "Map.to_list"
+  ; remap <%% @AddressMap.empty %%> "(Map [])"
+
+  (* ; remap <%% BV.verify_secret_vote_proof %%> "verify_secret_vote_proof" *)
+  (* ; remap <%% @BV.make_signup_msg %%> "make_signup_msg" *)
+  (* ; remap <%% @BV.make_commit_msg %%> "make_commit_msg" *)
+  (* ; remap <%% @BV.make_vote_msg %%> "make_vote_msg" *)
+  (* ; remap <%% @BV.secret_vote_proof %%> "secret_vote_proof" *)
+  (* ; remap <%% @BV.secret_key_proof %%> "secret_key_proof" *)
+  (* ; remap <%% @BV.hash_sk_data %%> "hash_sk_data" *)
+  (* ; remap <%% @BV.hash_sv_data %%> "hash_sv_data" *)
+
+  (* ; remap <%% @BV.handle_signup %%> "handle_signup" *)
+  (* ; remap <%% @BV.handle_commit_to_vote %%> "handle_commit_to_vote" *)
+  (* ; remap <%% @BV.handle_submit_vote %%> "handle_submit_vote" *)
+  (* ; remap <%% @BV.handle_tally_votes %%> "handle_tally_votes" *)
+
+
+  ; remap <%% modulus %%> modulus_
+  ; remap <%% BV.encodeA %%> "nat"
+  ; remap <%% BV.encodeNat %%> "nat"
+  
+
+  ; remap <%% @List.fold_left %%> "List.fold"
+  ; remap <%% @List.map %%> "List.map"
+  ; remap <%% @List.find %%> "List.find"
+  ; remap <%% @List.length %%> "List.length"
+  ; remap <%% @List.app %%> "List.append"
+  ; remap <%% @Serializable.serialize %%> "TODO_serialize"
+  ; remap <%% @Serializable.deserialize %%> "TODO_deserialize"
+  ].
+(** A translation table of constructors and some constants. The corresponding definitions will be extracted and renamed. *)
+Definition TT_rename : list (string * string):=
+  [ ("Some", "Some")
+  ; ("None", "None")
+  ; ("Zpos" ,"int")
+  ; ("Npos" ,"(fun (n:nat) -> n)")
+  ; ("Zneg" ,"-")
+  ; ("Z0" ,"0")
+  ; ("N0" ,"0")
+  ; ("xH" ,"0")
+  ; ("1" ,"1")
+  ; ("nil", "[]")
+  ; ("true", "true")
+  ; ("false", "false")
+  ; (string_of_kername <%% BV.State %%>, "State")  (* we add [storage] so it is printed without the prefix *) 
+  ; ("tt", "()")
+  ].
+
+(* Time MetaCoq Run (
+  t <- liquidity_prepare_extraction PREFIX TT_remap TT_rename to_inline BV_MODULE bv_env bv_init_nm bv_receive_nm ;;
+  tmDefinition BV_MODULE.(lmd_module_name) t
+  ).
+
+Print liquidity_boardroomvoting.  *)
 
 Time MetaCoq Run
      (t <- liquidity_extraction_specialize PREFIX TT_remap TT_rename to_inline BV_MODULE ;;
